Graph/Long.thy
@@ -1,0 +1,203 @@
+section \<open>java.lang.Long\<close>
+
+text \<open>
+Utility functions from the Long class that Graal occasionally makes use of.
+\<close>
+
+theory Long
+  imports ValueThms
+begin
+
+lemma negative_all_set_32:
+  "n < 32 \<Longrightarrow> bit (-1::int32) n"
+  apply transfer by auto
+
+(* TODO: better handle empty *)
+definition MaxOrZero :: "nat set \<Rightarrow> nat" where
+  "MaxOrZero s = (if s = {} then 0 else Max s)"
+
+definition MinOrHighest :: "nat set \<Rightarrow> nat \<Rightarrow> nat" where
+  "MinOrHighest s m = (if s = {} then m else Min s)"
+ 
+(* This is a different definition to Long.highestOneBit *)
+definition highestOneBit :: "('a::len) word \<Rightarrow> nat" where
+  "highestOneBit v = MaxOrZero {n . bit v n}"
+
+definition lowestOneBit :: "('a::len) word \<Rightarrow> nat" where
+  "lowestOneBit v = MinOrHighest {n . bit v n} (size v + 1)"
+
+lemma max_bit: "bit (v::('a::len) word) n \<Longrightarrow> n < size v"
+  by (simp add: bit_imp_le_length size_word.rep_eq)
+
+lemma max_set_bit: "MaxOrZero {n . bit (v::('a::len) word) n} \<le> Nat.size v"
+  using max_bit unfolding MaxOrZero_def
+  by force
+
+definition numberOfLeadingZeros :: "('a::len) word \<Rightarrow> nat" where
+  "numberOfLeadingZeros v = Nat.size v - highestOneBit v"
+
+lemma MaxOrZero_zero: "MaxOrZero {} = 0"
+  by (simp add: MaxOrZero_def)
+
+lemma MaxOrZero_max: "s \<noteq> {} \<Longrightarrow> MaxOrZero s = Max s"
+  by (simp add: MaxOrZero_def)
+
+lemma zero_no_bits:
+  "{n . bit 0 n} = {}"
+  by simp
+
+lemma "highestOneBit (0::64 word) = 0"
+  by (simp add: MaxOrZero_zero highestOneBit_def)
+
+lemma "numberOfLeadingZeros (0::64 word) = 64"
+  unfolding numberOfLeadingZeros_def
+  by (simp add: MaxOrZero_zero highestOneBit_def size64)
+
+lemma highestOneBit_top: "Max {highestOneBit (v::64 word)} \<le> 64"
+  unfolding highestOneBit_def
+  by (metis Max_singleton max_set_bit size64)
+
+lemma numberOfLeadingZeros_top: "Max {numberOfLeadingZeros (v::64 word)} \<le> 64"
+  unfolding numberOfLeadingZeros_def
+  by (simp add: size64)
+
+lemma leadingZerosAddHighestOne: "numberOfLeadingZeros v + highestOneBit v = Nat.size v"
+  by (simp add: highestOneBit_def max_set_bit numberOfLeadingZeros_def)
+
+definition numberOfTrailingZeros :: "('a::len) word \<Rightarrow> nat" where
+  "numberOfTrailingZeros v = lowestOneBit v - 1"
+
+lemma lowestOneBit_bot: "lowestOneBit (0::64 word) = 65"
+  unfolding lowestOneBit_def MinOrHighest_def
+  by (simp add: size64)
+
+lemma bit_zero_set_in_top: "bit (-1::'a::len word) 0"
+  by auto
+
+lemma nat_bot_set: "(0::nat) \<in> xs \<longrightarrow> (\<forall>x \<in> xs . 0 \<le> x)"
+  by fastforce
+
+lemma "numberOfTrailingZeros (0::64 word) = 64"
+  unfolding numberOfTrailingZeros_def
+  using lowestOneBit_bot by simp
+
+definition bitCount :: "('a::len) word \<Rightarrow> nat" where
+  "bitCount v = card {n . bit v n}"
+
+lemma "bitCount 0 = 0"
+  unfolding bitCount_def
+  by (metis card.empty zero_no_bits)
+
+lemma negone_set:
+  "bit (-1::('a::len) word) n \<longleftrightarrow> n < LENGTH('a)"
+  by simp
+
+lemma negone_all_bits:
+  "{n . bit (-1::('a::len) word) n} = {n . 0 \<le> n \<and> n < LENGTH('a)}"
+  using negone_set
+  by auto
+
+lemma bitCount_finite:
+  "finite {n . bit (v::('a::len) word) n}"
+  by simp
+
+lemma card_of_range:
+  "x = card {n . 0 \<le> n \<and> n < x}"
+  by simp
+
+lemma range_of_nat:
+  "{(n::nat) . 0 \<le> n \<and> n < x} = {n . n < x}"
+  by simp
+
+lemma finite_range:
+  "finite {n::nat . n < x}"
+  by simp
+
+lemma card_of_range_bound:
+  fixes x y :: nat
+  assumes "x > y"
+  shows "x - y = card {n . y < n \<and> n \<le> x}"
+proof -
+  have finite: "finite {n . y \<le> n \<and> n < x}"
+    by auto
+  have "x - y \<ge> 1"
+    using assms
+    by simp
+  show ?thesis
+    apply (cases "{n . y \<le> n \<and> n < x} = {}")
+    using assms apply blast
+    using assms finite apply auto sorry
+qed
+
+lemma "bitCount (-1::('a::len) word) = LENGTH('a)"
+  unfolding bitCount_def using card_of_range
+  by (metis (no_types, lifting) Collect_cong negone_all_bits)
+
+lemma bitCount_range:
+  fixes n :: "('a::len) word"
+  shows "0 \<le> bitCount n \<and> bitCount n \<le> Nat.size n"
+  unfolding bitCount_def
+  by (metis atLeastLessThan_iff bot_nat_0.extremum max_bit mem_Collect_eq subsetI subset_eq_atLeast0_lessThan_card)
+
+lemma zerosAboveHighestOne:
+  "n > highestOneBit a \<Longrightarrow> \<not>(bit a n)"
+  unfolding highestOneBit_def MaxOrZero_def
+  by (metis (mono_tags, lifting) Collect_empty_eq Max_ge bitCount_finite linorder_not_le mem_Collect_eq)
+
+lemma union_bit_sets:
+  fixes a :: "('a::len) word"
+  shows "{n . n < Nat.size a \<and> bit a n} \<union> {n . n < Nat.size a \<and> \<not>(bit a n)} = {n . n < Nat.size a}"
+  by fastforce
+
+lemma disjoint_bit_sets:
+  fixes a :: "('a::len) word"
+  shows "{n . n < Nat.size a \<and> bit a n} \<inter> {n . n < Nat.size a \<and> \<not>(bit a n)} = {}"
+  by blast
+
+lemma qualified_bitCount:
+  "bitCount v = card {n . n < Nat.size v \<and> bit v n}"
+  by (metis (no_types, lifting) Collect_cong bitCount_def max_bit)
+
+lemma card_eq:
+  assumes "finite x \<and> finite y \<and> finite z"
+  assumes "x \<union> y = z"
+  assumes "y \<inter> x = {}"
+  shows "card z - card y = card x"
+  using assms add_diff_cancel_right' card_Un_disjoint
+  by (metis inf.commute)
+
+lemma card_add:
+  assumes "finite x \<and> finite y \<and> finite z"
+  assumes "x \<union> y = z"
+  assumes "y \<inter> x = {}"
+  shows "card x + card y = card z"
+  using assms card_Un_disjoint
+  by (metis inf.commute)
+
+lemma intersect_bitCount_helper:
+  "card {n . n < Nat.size a} - bitCount a = card {n . n < Nat.size a \<and> \<not>(bit a n)}"
+proof -
+  have size_def: "Nat.size a = card {n . n < Nat.size a}"
+    using card_of_range by simp
+  have bitCount_def: "bitCount a = card {n . n < Nat.size a \<and> bit a n}"
+    using qualified_bitCount by auto
+  have disjoint: "{n . n < Nat.size a \<and> bit a n} \<inter> {n . n < Nat.size a \<and> \<not>(bit a n)} = {}"
+    using disjoint_bit_sets by auto
+  have union: "{n . n < Nat.size a \<and> bit a n} \<union> {n . n < Nat.size a \<and> \<not>(bit a n)} = {n . n < Nat.size a}"
+    using union_bit_sets by auto
+  show ?thesis
+    unfolding bitCount_def
+    apply (rule card_eq)
+    using finite_range apply simp
+    using union apply blast
+    using disjoint by simp
+qed
+
+lemma intersect_bitCount:
+  "Nat.size a - bitCount a = card {n . n < Nat.size a \<and> \<not>(bit a n)}"
+  using card_of_range intersect_bitCount_helper by auto
+
+hide_fact intersect_bitCount_helper
+
+end
+
